playing with merge sort

src/Collections/Sequences/MergeSort.dfy
@@ -12,7 +12,7 @@ module {:options "-functionSyntax:4"} Seq.MergeSort {
   import opened Relations
 
   //Splits a sequence in two, sorts the two subsequences using itself, and merge the two sorted sequences using `MergeSortedWith`
-  function MergeSortBy<T(!new)>(a: seq<T>, lessThanOrEq: (T, T) -> bool): (result :seq<T>)
+  function {:isolate_assertions} {:only} MergeSortBy<T(!new)>(a: seq<T>, lessThanOrEq: (T, T) -> bool): (result :seq<T>)
     requires TotalOrdering(lessThanOrEq)
     ensures multiset(a) == multiset(result)
     ensures SortedBy(result, lessThanOrEq)
@@ -30,6 +30,60 @@ module {:options "-functionSyntax:4"} Seq.MergeSort {
 
       MergeSortedWith(leftSorted, rightSorted, lessThanOrEq)
   }
+  // by method {
+  //   if |a| <= 1 {
+  //     return a;
+  //   } else {
+  //     var tmp := new T[|a|](i requires 0 <= i < |a| => a[i]);
+  //     MSort(tmp, lessThanOrEq);
+  //     return tmp[..];
+  //   }
+  // }
+
+  function {:only} Bar<T(!new)>(a: seq<T>, lessThanOrEq: (T, T) -> bool): (result :seq<T>)
+    requires TotalOrdering(lessThanOrEq)
+  {
+    MergeSortBy(a, lessThanOrEq)
+  }
+  by method {
+    if |a| <= 1 {
+      return a;
+    } else {
+      
+      var tmp := new T[|a|](i requires 0 <= i < |a| => a[i]);
+      MSort(tmp, lessThanOrEq);
+
+      
+      ghost var other := MergeSortBy(a, lessThanOrEq);
+      
+      calc {
+        multiset(tmp[..]);
+      ==
+        multiset(a);
+      ==
+        multiset(other);
+      }
+
+      assume false;
+
+      assert multiset(tmp[..]) == multiset(other);
+
+      assume false;
+
+      Foo(tmp[..], MergeSortBy(a, lessThanOrEq), lessThanOrEq);
+      return tmp[..];
+    }
+  }
+
+
+  lemma Foo<T(!new)>(s1: seq<T>, s2: seq<T>, lessThanOrEq: (T, T) -> bool)
+    requires TotalOrdering(lessThanOrEq)
+    requires SortedBy(s1, lessThanOrEq) && SortedBy(s2, lessThanOrEq)
+    requires multiset(s1) == multiset(s2)
+    ensures s1 == s2
+
+
+
 
   function {:tailrecursion} MergeSortedWith<T(!new)>(left: seq<T>, right: seq<T>, lessThanOrEq: (T, T) -> bool) : (result :seq<T>)
     requires SortedBy(left, lessThanOrEq)
@@ -53,5 +107,240 @@ module {:options "-functionSyntax:4"} Seq.MergeSort {
       assert right == [right[0]] + right[1..];
 
       [right[0]] + MergeSortedWith(left, right[1..], lessThanOrEq)
+  }
+
+  method {:isolate_assertions} MSort<T(!new)>(a: array<T>, lessThanOrEq: (T, T) -> bool, lo: nat := 0, hi: nat := a.Length)
+    requires 0 <= lo < hi <= a.Length
+    requires TotalOrdering(lessThanOrEq)
+    decreases hi - lo
+    reads a
+    modifies a
+    ensures multiset(a[..]) == multiset(old(a[..]))
+    ensures SortedBy(a[lo..hi], lessThanOrEq)
+    ensures a[0..lo] == old(a[0..lo])
+    ensures a[hi..] == old(a[hi..])
+    ensures a[lo..hi] == MergeSortBy(old(a[lo..hi]), lessThanOrEq)
+  {
+    var mid := lo + (hi - lo)/2;
+    if lo < mid {
+      MSort(a, lessThanOrEq, lo, mid);
+      MSort(a, lessThanOrEq, mid, hi);
+
+      Merge(a, lessThanOrEq, lo, mid, hi);
+    }
+  }
+
+  method {:isolate_assertions} Merge<T(!new)>(a: array<T>, lessThanOrEq: (T, T) -> bool, lo: nat, mid:nat, hi: nat)
+    requires TotalOrdering(lessThanOrEq)
+    requires 0 <= lo < mid <= hi <= a.Length
+    requires SortedBy(a[lo..mid], lessThanOrEq)
+    requires SortedBy(a[mid..hi], lessThanOrEq)
+    reads a
+    modifies a
+    ensures multiset(a[..]) == multiset(old(a[..]))
+    ensures SortedBy(a[lo..hi], lessThanOrEq)
+    ensures a[0..lo] == old(a[0..lo])
+    ensures a[hi..] == old(a[hi..])
+    // ensures a[lo..hi] == MergeSortedWith(old(a[lo..mid]), old(a[mid..hi]), lessThanOrEq)
+    ensures MergeSortBy(old(a[lo..hi]), lessThanOrEq) == a[lo..hi]
+  {
+    var fill := i requires 0 <= i < a.Length reads a => a[i];
+    var left, right :=
+      new T[mid - lo](i requires 0 <= i < a.Length - lo reads a  => a[lo + i]),
+      new T[hi - mid](i requires 0 <= i < a.Length - mid reads a => a[mid + i]);
+
+    var i, l, r := lo,0,0;
+
+    label BEFORE_LOOP:
+
+    assert a[lo..mid] == left[..];
+    assert a[mid..hi] == right[..];
+
+    assert a[..i] + left[l..] + right[r..] + a[hi..] == a[..] == old(a[..]);
+
+    while i < hi
+      decreases hi - i
+      modifies a
+
+      invariant 0 <= lo <= i <= hi <= a.Length
+      invariant 0 <= l <= left.Length
+      invariant 0 <= r <= right.Length
+
+      invariant
+        && lo < i
+        && r < right.Length
+        ==>
+          && lessThanOrEq(a[i-1], right[r])
+
+      invariant
+        && lo < i
+        && l < left.Length
+        ==>
+          && lessThanOrEq(a[i-1], left[l])
+
+      invariant SortedBy(a[lo..i], lessThanOrEq)
+
+      invariant unchanged@BEFORE_LOOP(left)
+      invariant unchanged@BEFORE_LOOP(right)
+      invariant SortedBy(left[..], lessThanOrEq)
+      invariant SortedBy(right[..], lessThanOrEq)
+
+      invariant lo + l + r == i
+
+      invariant a[0..lo] == old(a[0..lo])
+      invariant a[i..] == old(a[i..])
+      invariant multiset(a[..i] + left[l..] + right[r..] + a[hi..]) == multiset(old(a[..]))
+
+
+
+
+      // invariant
+      //   assert old(a[lo..lo+l]) == left[..l];
+      //   a[lo..i] == MergeSortedWith(old(a[lo..lo+l]), old(a[mid..mid+r]), lessThanOrEq)
+
+      invariant a[lo..i] == MergeSortedWith(left[..l], right[..r], lessThanOrEq)
+
+    {
+
+      if l < left.Length && r < right.Length {
+        if lessThanOrEq(left[l], right[r]) {
+          a[i] := left[l];
+
+          PushStillSortedBy(a, lo, i, lessThanOrEq);
+          l := l + 1;
+
+          assert l < left.Length ==> lessThanOrEq(a[i], left[l]) by {
+            assert a[i] == left[l-1];
+            if l < left.Length {
+              assert lessThanOrEq(left[l-1], left[l]) by {
+                assert forall i, j | 0 <= i < j < |left[..]| :: lessThanOrEq(left[..][i], left[..][j]);
+                assert 0 <= l-1 < l < |left[..]|;
+              }
+            }
+          }
+          assert lessThanOrEq(a[i], right[r]);
+
+          assert multiset(a[..i+1] + left[l..] + right[r..] + a[hi..]) == multiset(old(a[..])) by {
+            calc {
+              a[..i] + left[l-1..] + right[r..] + a[hi..];
+            == {assert [left[l-1]] + left[l..] == left[l-1..];}
+              a[..i] + ([left[l-1]] + left[l..]) + right[r..] + a[hi..];
+            == {assert a[i] == left[l-1];}
+              a[..i] + ([a[i]] + left[l..]) + right[r..] + a[hi..];
+            == {assert a[..i] + ([a[i]] + left[l..]) == (a[..i] + [a[i]]) + left[l..];}
+              (a[..i] + [a[i]]) + left[l..] + right[r..] + a[hi..];
+            == {assert a[..i] +[a[i]] == a[..i+1];}
+              a[..i+1] + left[l..] + right[r..] + a[hi..];
+            }
+          }
+
+        } else {
+          a[i] := right[r];
+
+          PushStillSortedBy(a, lo, i, lessThanOrEq);
+          r := r + 1;
+
+          assert r < right.Length ==> lessThanOrEq(a[i], right[r]) by {
+            assert a[i] == right[r-1];
+            if r < right.Length {
+              assert lessThanOrEq(right[r-1], right[r]) by {
+                assert forall i, j | 0 <= i < j < |right[..]| :: lessThanOrEq(right[..][i], right[..][j]);
+                assert 0 <= r-1 < r < |right[..]|;
+              }
+            }
+          }
+          assert lessThanOrEq(a[i], left[l]);
+
+          assert multiset(a[..i+1] + left[l..] + right[r..] + a[hi..]) == multiset(old(a[..])) by {
+            calc {
+              a[..i] + left[l..] + right[r-1..] + a[hi..];
+            == {assert [right[r-1]] + right[r..] == right[r-1..];}
+              a[..i] + left[l..] + ([right[r-1]] + right[r..]) + a[hi..];
+            == {assert a[i] == right[r-1];}
+              a[..i] + left[l..] + ([a[i]] + right[r..]) + a[hi..];
+            }
+          }
+        }
+
+      } else if l == left.Length && r < right.Length {
+        // We reached the end of left,
+        // all of right is in order,
+        // we just need to move it in.
+        a[i] := right[r];
+
+        PushStillSortedBy(a, lo, i, lessThanOrEq);
+        r := r + 1;
+
+        assert r < right.Length ==> lessThanOrEq(a[i], right[r]);
+
+        assert multiset(a[..i+1] + left[l..] + right[r..] + a[hi..]) == multiset(old(a[..])) by {
+          calc {
+            a[..i] + left[l..] + right[r-1..] + a[hi..];
+          == {assert [right[r-1]] + right[r..] == right[r-1..];}
+            a[..i] + left[l..] + ([right[r-1]] + right[r..]) + a[hi..];
+          == {assert a[i] == right[r-1];}
+            a[..i] + left[l..] + ([a[i]] + right[r..]) + a[hi..];
+          }
+        }
+
+      } else if r == right.Length && l < left.Length {
+        // We reached the end of right
+        // all of left is in order,
+        // we just need to move it in.
+        a[i] := left[l];
+
+        PushStillSortedBy(a, lo, i, lessThanOrEq);
+        l := l + 1;
+
+        assert l < left.Length ==> lessThanOrEq(a[i], left[l]) by {
+          assert a[i] == left[l-1];
+        }
+
+        assert multiset(a[..i+1] + left[l..] + right[r..] + a[hi..]) == multiset(old(a[..])) by {
+          calc {
+            a[..i] + left[l-1..] + right[r..] + a[hi..];
+          == {assert [left[l-1]] + left[l..] == left[l-1..];}
+            a[..i] + ([left[l-1]] + left[l..]) + right[r..] + a[hi..];
+          == {assert a[i] == left[l-1];}
+            a[..i] + ([a[i]] + left[l..]) + right[r..] + a[hi..];
+          == {assert a[..i] + ([a[i]] + left[l..]) == (a[..i] + [a[i]]) + left[l..];}
+            (a[..i] + [a[i]]) + left[l..] + right[r..] + a[hi..];
+          == {assert a[..i] +[a[i]] == a[..i+1];}
+            a[..i+1] + left[l..] + right[r..] + a[hi..];
+          }
+        }
+      } else {
+        // There is never a case where
+        // we are not pulling from right or left
+        assert false;
+      }
+
+      i := i + 1;
+
+      assert a[i..] == old(a[i..]);
+    }
+
+    assert multiset(a[..]) == multiset(old(a[..])) by {
+      assert multiset(a[..i] + left[l..] + right[r..] + a[hi..]) == multiset(old(a[..]));
+      assert a[..] == a[..i] + left[l..] + right[r..] + a[hi..];
+    }
+
+  }
+
+  lemma PushStillSortedBy<T(!new)>(a: array<T>, lo:nat, i: nat, lessThan: (T, T) -> bool)
+    requires 0 <= lo <= i < a.Length
+    requires SortedBy(a[lo..i], lessThan)
+    requires |a[lo..i]| == 0 || lessThan(a[lo..i][|a[lo..i]| - 1], a[i])
+    requires TotalOrdering(lessThan)
+    ensures SortedBy(a[lo..i + 1], lessThan)
+    ensures lo < i ==> lessThan(a[i - 1], a[i])
+  {}
+
+  method ToArray<T(!new)>(xs: seq<T>) returns (a: array<T>)
+    ensures fresh(a)
+    ensures a.Length == |xs|
+    ensures forall i :: 0 <= i < |xs| ==> a[i] == xs[i]
+  {
+    a := new T[|xs|](i requires 0 <= i < |xs| => xs[i]);
   }
 }
